rearranging some things and some small cleanups

steel/Veritas.SingleThreadSimulation.fst
@@ -2,7 +2,6 @@ module Veritas.SingleThreadSimulation
 open FStar.Ghost
 module I = Veritas.Intermediate.Verify
 module S = Veritas.Steel.VerifierModel
-module VCache = Veritas.Steel.VCache
 module VCfg = Veritas.Intermediate.VerifierConfig
 module IStore = Veritas.Intermediate.Store
 module MSH = Veritas.MultiSetHashDomain
@@ -33,13 +32,13 @@ let bv_of_u256 (i:S_Types.u256) : BV.bv_t 256 =
 let bitvec_of_u256 (i:S_Types.u256) : FStar.BitVector.bv_t 256 =
   Seq.seq_of_list (BV.bv2list (bv_of_u256 i))
 
-assume
-val bitvec_of_u256_inj (i j:_)
+let bitvec_of_u256_inj (i j:_)
   : Lemma
     (ensures bitvec_of_u256 i == bitvec_of_u256 j ==>
              i == j)
     [SMTPat (bitvec_of_u256 i);
      SMTPat (bitvec_of_u256 j)]
+  = admit()
 
 [@@"opaque_to_smt"]
 let int_of_u256 (i:S_Types.u256) : int =
@@ -73,18 +72,24 @@ let rec bool_list_as_bin_tree (l:list bool)
     | true :: rest -> LeftChild (bool_list_as_bin_tree rest)
     | false :: rest -> RightChild (bool_list_as_bin_tree rest)
 
-[@@"opaque_to_smt"]
-let s_key_as_i_key (s_key:S_Types.key)
-  : Veritas.BinTree.bin_tree_node
-  = let (| l, m |) = key_as_list s_key in
-    bool_list_as_bin_tree l
-
 let related_key (s_key:S_Types.key)
                 (i_key:Veritas.Key.key)
   = let open S_Types in
     let (| l, m |) = key_as_list s_key in
     bool_list_as_bin_tree l == i_key /\
     L.for_all (( = ) false) m
+
+[@@"opaque_to_smt"]
+let lift_key (s:S_Types.key)
+  : option (s':Veritas.Key.key{related_key s s'})
+  = let open S_Types in
+    let (| l, m |) = key_as_list s in
+    if L.for_all (( = ) false) m
+    then let k = bool_list_as_bin_tree l in
+         if BinTree.depth k < Key.key_size
+         then Some k
+         else None
+    else None
 
 let related_key_inj (k0 k1:_) (m0 m1:_)
   : Lemma
@@ -246,13 +251,14 @@ let lift_slot #vcfg (s:S_Types.slot_id)
     then None
     else Some i_slot
 
-let lift_key (s:S_Types.key)
-  : option (s':Veritas.Key.key{related_key s s'})
-  = admit()
+let related_slots #vcfg  (slot_s:S_Types.slot_id)
+                         (slot_i:VC.slot_id vcfg)
+  = U16.v slot_s == slot_i
 
-let lift_value (s:S_Types.value)
+
+assume
+val lift_value (s:S_Types.value)
   : option (Veritas.Record.value)
-  = admit()
 
 let lift_record (s:S_Types.record)
   : option Veritas.Record.record
@@ -269,13 +275,14 @@ let lift_vlog_entry_get_put #vcfg (e:S_Types.vlog_entry_get_put)
             Veritas.Record.data_value)
   = let open S_Types in
     let i_slot = lift_slot #vcfg e.vegp_s in
-    let i_key = s_key_as_i_key e.vegp_k in
+    let i_key = lift_key e.vegp_k in
     let i_data = lift_data_value e.vegp_v in
     if None? i_slot
-    ||  Veritas.BinTree.depth i_key <> Veritas.Key.key_size
+    ||  None? i_key
+    ||  Veritas.BinTree.depth (Some?.v i_key) <> Veritas.Key.key_size
     ||  U16.v e.vegp_k.significant_digits <> Veritas.Key.key_size
     then None
-    else Some (Some?.v i_slot, i_key, i_data)
+    else Some (Some?.v i_slot, Some?.v i_key, i_data)
 
 let lift_log_entry #vcfg (v:S_Types.vlog_entry)
   : option (IL.logS_entry vcfg)
@@ -350,128 +357,11 @@ let related_lift_vlog_entry_get_put #vcfg (e:S_Types.vlog_entry_get_put)
       related_key e.vegp_k k /\
       related_value (V_dval e.vegp_v) (DVal v)
     ))
-  = admit()
-
-#push-options "--fuel 0 --ifuel 1 --z3rlimit_factor 4"
-////////////////////////////////////////////////////////////////////////////////
-// VGET
-////////////////////////////////////////////////////////////////////////////////
-let related_vget (#vcfg: _)
-                 (tsm:S.thread_state_model)
-                 (vtls:I.vtls vcfg)
-                 (v:S_Types.vlog_entry { S_Types.Ve_Get? v })
-  : Lemma
-    (requires
-      Some? (lift_log_entry #vcfg v) /\
-      related_states tsm vtls /\
-      I.Valid? vtls)
-    (ensures (
-      let open S_Types in
-      let open IL in
-      let gp = Ve_Get?._0 v in
-      let Some (Get_S s k d) = lift_log_entry #vcfg v in
-      (S.vget_model tsm gp.vegp_s gp.vegp_k (V_dval gp.vegp_v))
-        `related_states`
-      (I.vget s k d vtls)))
-   =
-    let open Veritas.Record in
+  = let open Veritas.Record in
     let open S_Types in
-    let open IL in
-    let open S in
-    let gp = Ve_Get?._0 v in
-    let Some (Get_S s k d) = lift_log_entry #vcfg v in
-    related_lift_vlog_entry_get_put #vcfg gp;
-    let tsm' = S.vget_model tsm gp.vegp_s gp.vegp_k (V_dval gp.vegp_v) in
-    let vtls' = I.vget s k d vtls in
-    let I.Valid id st clock hadd hevict = vtls in
-    match model_get_record tsm gp.vegp_s with
-    | None -> ()
-    | Some r ->
-      let Some s = IStore.get_slot st s in
-      let kk = IStore.VStoreE?.k s in
-      let vv = IStore.VStoreE?.v s in
-      assert (related_key (r.S.record_key) kk);
-      assert (related_value (r.S.record_value) vv);
-      related_key_inj gp.vegp_k (r.S.record_key)
-                      k kk;
-      related_value_inj (V_dval gp.vegp_v)
-                        r.S.record_value
-                        (DVal d)
-                        vv
-
-////////////////////////////////////////////////////////////////////////////////
-// VPUT
-////////////////////////////////////////////////////////////////////////////////
-
-let related_slots #vcfg  (slot_s:S_Types.slot_id)
-                         (slot_i:VC.slot_id vcfg)
-  = U16.v slot_s == slot_i
-
-let update_entry #vcfg
-                 (i_record:IStore.vstore_entry vcfg)
-                 (v:Veritas.Record.value_type_of (IStore.VStoreE?.k i_record))
-  : IStore.vstore_entry vcfg
-  = let IStore.VStoreE kk _ am l_in_store r_in_store p = i_record in
-    IStore.VStoreE kk v am l_in_store r_in_store p
-
-let istore_upd_value #vcfg
-                     (st:IStore.vstore vcfg)
-                     (s:IStore.inuse_slot_id st)
-                     (d:Veritas.Record.value_type_of (IStore.stored_key st s))
-  : Lemma
-    (requires
-      Some? (IStore.get_slot st s))
-    (ensures (
-      let Some e = IStore.get_slot st s in
-      IStore.update_value st s d `Seq.equal`
-      Seq.upd st s (Some (update_entry e d))))
-    [SMTPat (IStore.update_value st s d)]
-  = let open IStore in
-    let st' = IStore.update_value st s d in
-    //just need to trigger a rewrite get_slot into seq.index
-    assert (forall i. i <> s ==> get_slot st i == get_slot st' i /\ Seq.index st i == Seq.index st' i)
-
-let related_vput (#vcfg: _)
-                 (tsm:S.thread_state_model)
-                 (vtls:I.vtls vcfg)
-                 (v:S_Types.vlog_entry { S_Types.Ve_Put? v })
-  : Lemma
-    (requires
-      Some? (lift_log_entry #vcfg v) /\
-      related_states tsm vtls /\
-      I.Valid? vtls)
-    (ensures (
-      let open S_Types in
-      let open IL in
-      let gp = Ve_Put?._0 v in
-      let Some (Put_S s k d) = lift_log_entry #vcfg v in
-      (S.vput_model tsm gp.vegp_s gp.vegp_k (V_dval gp.vegp_v))
-        `related_states`
-      (I.vput s k d vtls)))
-   = let open Veritas.Record in
-     let open S_Types in
-     let open IL in
-     let open S in
-     let gp = Ve_Put?._0 v in
-     let Some (Put_S s k d) = lift_log_entry #vcfg v in
-     related_lift_vlog_entry_get_put #vcfg gp;
-     let tsm' = S.vput_model tsm gp.vegp_s gp.vegp_k (V_dval gp.vegp_v) in
-     let vtls' = I.vput s k d vtls in
-     let I.Valid id st clock hadd hevict = vtls in
-     match model_get_record tsm gp.vegp_s with
-     | None -> ()
-     | Some r ->
-       let Some entry = IStore.get_slot st s in
-       let IStore.VStoreE kk vv am l_in_store r_in_store p = entry in
-       related_key_inj gp.vegp_k (r.S.record_key)
-                      k kk;
-       if k <> kk then ()
-       else istore_upd_value st s (DVal d)
-
-////////////////////////////////////////////////////////////////////////////////
-// VADDM
-////////////////////////////////////////////////////////////////////////////////
-let z_thread_id : S_Types.thread_id = 0us
+    let Some (s, k, v) = lift_vlog_entry_get_put #vcfg e in
+    assert (related_key e.vegp_k k);
+    admit()
 
 let related_desc_dir (b:bool) (d:Veritas.BinTree.bin_tree_dir) =
   b = Veritas.BinTree.Left? d
@@ -677,185 +567,6 @@ let related_update_merkle_value (s_v:_)
      SMTPat (Verifier.update_merkle_value i_v i_d i_k i_h b)]
   = admit()
 
-#push-options "--z3rlimit_factor 8 --query_stats --ifuel 1"
-
-let vaddm_basic_preconditions tsm s_s s_k s_v s_s' s_k' s_v'
-                              s_mv' s_d s_dh' s_h
-                              #vcfg (vtls:I.vtls vcfg{I.Valid? vtls})
-                              i_s i_k i_v i_s' i_k' i_v'
-                              i_mv' i_d i_dh' i_h
-  = let st = (I.thread_store vtls) in
-    related_states tsm vtls /\
-    related_slots #vcfg s_s i_s /\
-    related_key s_k i_k /\
-    related_value s_v i_v /\
-    related_slots #vcfg s_s' i_s' /\
-    related_key s_k' i_k' /\
-    related_value s_v' i_v' /\
-    (S.is_proper_descendent s_k s_k' /\
-     Some? (S.model_get_record tsm s_s') /\
-     S.is_value_of s_k s_v /\
-     (let r = Some?.v (S.model_get_record tsm s_s') in
-      r.S.record_key == s_k' /\
-      r.S.record_value == s_v') /\
-    Some s_mv' == S.to_merkle_value s_v' /\
-    s_d == S.desc_dir s_k s_k' /\
-    s_dh' == S.desc_hash_dir s_mv' s_d /\
-    s_h == S.hashfn s_v) /\
-    (i_s <> i_s' /\
-     not (IStore.empty_slot st i_s') /\
-     BinTree.is_proper_desc i_k i_k' /\
-     not (IStore.inuse_slot st i_s) /\
-     Record.is_value_of i_k i_v /\
-     IStore.stored_key st i_s' == i_k' /\
-     IStore.stored_value st i_s' == i_v' /\
-     i_mv'== Veritas.Record.to_merkle_value i_v' /\
-     i_d == Veritas.BinTree.desc_dir i_k i_k' /\
-     i_dh' == Veritas.Record.desc_hash_dir i_mv' i_d /\
-     i_h == Veritas.Hash.hashfn i_v)
-
-let related_vaddm_no_child tsm s_s s_k s_v s_s' s_k' s_v' s_mv' s_d s_dh' s_h
-                           #vcfg (vtls:I.vtls vcfg{I.Valid? vtls})
-                           i_s i_k i_v i_s' i_k' i_v' i_mv' i_d i_dh' i_h
-  : Lemma
-    (requires vaddm_basic_preconditions
-                   tsm s_s s_k s_v s_s' s_k' s_v'
-                   s_mv' s_d s_dh' s_h
-                   vtls i_s i_k i_v i_s' i_k' i_v'
-                   i_mv' i_d i_dh' i_h /\
-              S_Types.Dh_vnone? s_dh')
-    (ensures
-      (S.vaddm_model tsm s_s S_Types.({record_key = s_k; record_value = s_v}) s_s' z_thread_id
-        `related_states`
-      (I.vaddm i_s (i_k, i_v) i_s' vtls)))
-  = let open Veritas.Record in
-    let open S_Types in
-    let open IL in
-    let open S in
-    related_key_proper_descendent s_k s_k' i_k i_k';
-    let tsm' =
-      S.vaddm_model
-        tsm
-        s_s
-        S_Types.({record_key = s_k; record_value = s_v})
-        s_s'
-        z_thread_id
-    in
-    let vtls' = I.vaddm i_s (i_k, i_v) i_s' vtls in
-    let st = (I.thread_store vtls) in
-    let s_r' = Some?.v (S.model_get_record tsm s_s') in
-    let Some i_r' = IStore.get_slot st i_s' in
-    related_hashfn s_v i_v;
-    related_desc_hash_dir s_mv' s_d i_mv' i_d;
-    assert (i_dh' == Empty);
-    related_init_value s_k i_k;
-    if s_v = S.init_value s_k
-    then (
-      assert (i_v = Veritas.Record.init_value i_k);
-      points_to_some_slot_related tsm st s_s' s_d i_d;
-      if S.points_to_some_slot tsm s_s' s_d
-      then ()
-      else (
-        madd_to_store_related tsm st s_s s_k s_v s_s' s_d i_s i_k i_v i_s' i_d;
-        let tsm1 = S.model_madd_to_store tsm s_s s_k s_v s_s' s_d in
-        let st1 = IStore.madd_to_store st i_s i_k i_v i_s' i_d in
-        assert (related_stores tsm1.S.model_store st1);
-
-        related_update_merkle_value
-                  (S_Types.V_mval?._0 s_v') s_d s_k s_h
-                  (Record.MVal?.v i_v') i_d i_k i_h false
-      )
-    )
-    else (
-      assert (i_v <> Veritas.Record.init_value i_k)
-    )
-
-let related_vaddm_some_child tsm s_s s_k s_v s_s' s_k' s_v' s_mv' s_d s_dh' s_h
-                           #vcfg (vtls:I.vtls vcfg{I.Valid? vtls})
-                           i_s i_k i_v i_s' i_k' i_v' i_mv' i_d i_dh' i_h
-  : Lemma
-    (requires vaddm_basic_preconditions
-                   tsm s_s s_k s_v s_s' s_k' s_v'
-                   s_mv' s_d s_dh' s_h
-                   vtls i_s i_k i_v i_s' i_k' i_v'
-                   i_mv' i_d i_dh' i_h /\
-              S_Types.Dh_vsome? s_dh')
-    (ensures
-      (S.vaddm_model tsm s_s S_Types.({record_key = s_k; record_value = s_v}) s_s' z_thread_id
-        `related_states`
-      (I.vaddm i_s (i_k, i_v) i_s' vtls)))
-  = let open Veritas.Record in
-    let open S_Types in
-    let open IL in
-    let open S in
-    related_key_proper_descendent s_k s_k' i_k i_k';
-    let tsm' =
-      S.vaddm_model
-        tsm
-        s_s
-        S_Types.({record_key = s_k; record_value = s_v})
-        s_s'
-        z_thread_id
-    in
-    let vtls' = I.vaddm i_s (i_k, i_v) i_s' vtls in
-    let st = (I.thread_store vtls) in
-    let s_r' = Some?.v (S.model_get_record tsm s_s') in
-    let Some i_r' = IStore.get_slot st i_s' in
-    related_hashfn s_v i_v;
-    related_desc_hash_dir s_mv' s_d i_mv' i_d;
-    let Dh_vsome {dhd_key=s_k2; dhd_h=s_h2; evicted_to_blum = s_b2} = s_dh' in
-    let Desc i_k2 i_h2 i_b2 = i_dh' in
-    related_key_inj s_k s_k2 i_k i_k2;
-    if s_k2 = s_k
-    then (
-       points_to_some_slot_related tsm st s_s' s_d i_d;
-       if not (s_h2 = s_h && s_b2 = Vfalse)
-       then ()
-       else if points_to_some_slot tsm s_s' s_d
-       then ()
-       else (
-         madd_to_store_related tsm st s_s s_k s_v s_s' s_d i_s i_k i_v i_s' i_d
-       )
-    )
-    else (
-      related_init_value s_k i_k;
-      if s_v <> S.init_value s_k
-      then ()
-      else (
-        related_key_proper_descendent s_k2 s_k i_k2 i_k;
-        if not (S.is_proper_descendent s_k2 s_k)
-        then ()
-        else (
-          let Some s_mv = S.to_merkle_value s_v in
-          let s_d2 = S.desc_dir s_k2 s_k in
-          let Record.MVal i_mv = i_v in
-          let i_d2 = BinTree.desc_dir i_k2 i_k in
-          assert (related_desc_dir s_d2 i_d2);
-          related_update_merkle_value
-            s_mv s_d2 s_k2 s_h2
-            i_mv i_d2 i_k2 i_h2 i_b2;
-          let i_mv_upd = Verifier.update_merkle_value i_mv i_d2 i_k2 i_h2 i_b2 in
-          let s_mv_upd = S.update_merkle_value s_mv s_d2 s_k2 s_h2 (s_b2=Vtrue) in
-          related_update_merkle_value
-            s_mv' s_d s_k s_h
-            i_mv' i_d i_k i_h false;
-          let i_v'_upd = Verifier.update_merkle_value i_mv' i_d i_k i_h false in
-          let s_v'_upd = S.update_merkle_value s_mv' s_d s_k s_h false in
-          points_to_some_slot_related
-            tsm st s_s' s_d i_d;
-          if S.points_to_some_slot tsm s_s' s_d
-          then
-            madd_to_store_split_related tsm st
-              s_s s_k (V_mval s_mv_upd) s_s' s_d s_d2
-              i_s i_k (MVal i_mv_upd) i_s' i_d i_d2
-          else
-            madd_to_store_related tsm st
-               s_s s_k (V_mval s_mv_upd) s_s' s_d
-               i_s i_k (MVal i_mv_upd) i_s' i_d
-        )
-      )
-    )
-
 let value_of_related (s_k:_) (s_v:_)
                      (i_k:_) (i_v:_)
   : Lemma
@@ -867,98 +578,6 @@ let value_of_related (s_k:_) (s_v:_)
       Record.is_value_of i_k i_v)
   = admit()
 
-let related_vaddm (#vcfg: _)
-                  (tsm:S.thread_state_model)
-                  (vtls:I.vtls vcfg)
-                  (v:S_Types.vlog_entry)
-  : Lemma
-    (requires
-      S_Types.Ve_AddM? v == true /\
-      Some? (lift_log_entry #vcfg v) == true /\
-      related_states tsm vtls /\
-      I.Valid? vtls == true)
-    (ensures (
-      let open S_Types in
-      let open IL in
-      let addm = Ve_AddM?._0 v in
-      let Some (AddM_S s r s') = lift_log_entry #vcfg v in
-      (S.vaddm_model tsm addm.veam_s addm.veam_r addm.veam_s2 z_thread_id
-        `related_states`
-      (I.vaddm s r s' vtls))))
-  = let open Veritas.Record in
-    let open S_Types in
-    let open IL in
-    let open S in
-    let addm = Ve_AddM?._0 v in
-    let Some (AddM_S i_s i_r i_s') = lift_log_entry #vcfg v in
-    related_lift_log_entry_addm #vcfg v;
-    let s_s = addm.veam_s in
-    let s_r = addm.veam_r in
-    let s_s' = addm.veam_s2  in
-    let tsm' = S.vaddm_model tsm s_s s_r s_s' z_thread_id in
-    let vtls' = I.vaddm i_s i_r i_s' vtls in
-    let I.Valid id st clock hadd hevict = vtls in
-    match model_get_record tsm s_s' with
-    | None -> ()
-    | Some s_r' ->
-      assert (not (IStore.empty_slot st i_s'));
-      let Some i_r' = IStore.get_slot st i_s' in
-      assert (related_record s_r' i_r');
-      let s_k = addm.veam_r.S_Types.record_key in
-      let s_v = addm.veam_r.S_Types.record_value in
-      let s_k' = s_r'.record_key in
-      let s_v' = s_r'.record_value in
-      let i_k, i_v = i_r in
-      let i_k' = IStore.stored_key st i_s' in
-      let i_v' = IStore.stored_value st i_s' in
-      if i_s = i_s'
-      then (
-        assert (vtls' == I.Failed);
-        assert (tsm'.model_failed)
-        //At the TSM level, we do not explicitly check that s <> s'
-        //but it follows anyway, since if s' is not in the store it fails
-        //and if s' is in the store then s must not be in the store
-      ) else (
-        related_key_proper_descendent s_k s_k' i_k i_k';
-        if not (S.is_proper_descendent s_k s_k')
-        then ()
-        else if Some? (model_get_record tsm s_s)
-        then ()
-        else (
-          value_of_related s_k s_v i_k i_v;
-          if not (S.is_value_of s_k s_v)
-          then ()
-          else (
-            assert (Veritas.Record.is_value_of i_k i_v);
-            assert (Veritas.Record.MVal? i_v');
-            assert (related_value s_v' i_v');
-            assert (S_Types.V_mval? s_v');
-            let i_mv' = Veritas.Record.to_merkle_value i_v' in
-            let i_d = Veritas.BinTree.desc_dir i_k i_k' in
-            let i_dh' = Veritas.Record.desc_hash_dir i_mv' i_d in
-            let i_h = Veritas.Hash.hashfn i_v in
-            let Some s_mv' = S.to_merkle_value s_v' in
-            let s_d = S.desc_dir s_k s_k' in
-            let s_dh' = S.desc_hash_dir s_mv' s_d in
-            let s_h = S.hashfn s_v in
-            related_hashfn s_v i_v;
-            assert (related_hashes (bitvec_of_u256 s_h) i_h);
-            related_desc_hash_dir s_mv' s_d i_mv' i_d;
-            match s_dh' with
-            | S_Types.Dh_vnone _ ->
-              related_vaddm_no_child
-                tsm s_s s_k s_v s_s' s_k' s_v' s_mv' s_d s_dh' s_h
-              vtls i_s i_k i_v i_s' i_k' i_v' i_mv' i_d i_dh' i_h
-            | _ ->
-              related_vaddm_some_child
-                tsm s_s s_k s_v s_s' s_k' s_v' s_mv' s_d s_dh' s_h
-              vtls i_s i_k i_v i_s' i_k' i_v' i_mv' i_d i_dh' i_h
-          )
-        )
-      )
-////////////////////////////////////////////////////////////////////////////////
-// vaddb
-////////////////////////////////////////////////////////////////////////////////
 let related_lift_log_entry_addb #vcfg (e:S_Types.vlog_entry { S_Types.Ve_AddB? e})
   : Lemma
     (requires Some? (lift_log_entry #vcfg e))
@@ -1030,6 +649,434 @@ let badd_to_store_related #vcfg (tsm:_) (vtls:I.vtls vcfg{I.Valid? vtls})
       related_states tsm' vtls'))
   = admit()
 
+let timestamp_lt_related  (s_t s_t':S_Types.timestamp)
+                          (i_t i_t':MSH.timestamp)
+  : Lemma
+    (requires
+      related_clocks s_t i_t /\
+      related_clocks s_t' i_t')
+    (ensures
+      MSH.ts_lt i_t i_t' <==>
+      S.timestamp_lt s_t s_t')
+    [SMTPat (related_clocks s_t i_t);
+     SMTPat (related_clocks s_t' i_t')]
+  = admit()
+
+let is_root_related (s_k:_) (i_k:Veritas.Key.key)
+  : Lemma
+    (requires
+      related_key s_k i_k)
+    (ensures
+      S.is_root s_k <==> i_k=BinTree.Root)
+    [SMTPat (related_key s_k i_k);
+     SMTPat (S.is_root s_k)]
+  = admit()
+
+let model_update_hash_related (s_h:_) (s_k:_) (s_v:_) (s_t:_) (s_j:_)
+                              (i_h:_) (i_k:_) (i_v:_) (i_t:_) (i_j:_)
+  : Lemma
+    (requires
+      related_hashes s_h i_h /\
+      related_key s_k i_k /\
+      related_value s_v i_v /\
+      related_thread_id s_j i_j /\
+      related_clocks s_t i_t)
+    (ensures (
+      let open S_Types in
+      related_hashes
+        (S.model_update_hash s_h ({record_key=s_k; record_value=s_v}) s_t s_j)
+        (MultiSetHash.ms_hashfn_upd (MSH.MHDom (i_k, i_v) i_t i_j) i_h)))
+    [SMTPat (S.model_update_hash s_h ({S_Types.record_key=s_k; S_Types.record_value=s_v}) s_t s_j);
+    SMTPat (MultiSetHash.ms_hashfn_upd (MSH.MHDom (i_k, i_v) i_t i_j) i_h)]
+  = admit()
+
+
+#push-options "--fuel 0 --ifuel 1 --z3rlimit_factor 4"
+////////////////////////////////////////////////////////////////////////////////
+// VGET
+////////////////////////////////////////////////////////////////////////////////
+let related_vget (#vcfg: _)
+                 (tsm:S.thread_state_model)
+                 (vtls:I.vtls vcfg)
+                 (v:S_Types.vlog_entry { S_Types.Ve_Get? v })
+  : Lemma
+    (requires
+      Some? (lift_log_entry #vcfg v) /\
+      related_states tsm vtls /\
+      I.Valid? vtls)
+    (ensures (
+      let open S_Types in
+      let open IL in
+      let gp = Ve_Get?._0 v in
+      let Some (Get_S s k d) = lift_log_entry #vcfg v in
+      (S.vget_model tsm gp.vegp_s gp.vegp_k (V_dval gp.vegp_v))
+        `related_states`
+      (I.vget s k d vtls)))
+   =
+    let open Veritas.Record in
+    let open S_Types in
+    let open IL in
+    let open S in
+    let gp = Ve_Get?._0 v in
+    let Some (Get_S s k d) = lift_log_entry #vcfg v in
+    related_lift_vlog_entry_get_put #vcfg gp;
+    let tsm' = S.vget_model tsm gp.vegp_s gp.vegp_k (V_dval gp.vegp_v) in
+    let vtls' = I.vget s k d vtls in
+    let I.Valid id st clock hadd hevict = vtls in
+    match model_get_record tsm gp.vegp_s with
+    | None -> ()
+    | Some r ->
+      let Some s = IStore.get_slot st s in
+      let kk = IStore.VStoreE?.k s in
+      let vv = IStore.VStoreE?.v s in
+      assert (related_key (r.S.record_key) kk);
+      assert (related_value (r.S.record_value) vv);
+      related_key_inj gp.vegp_k (r.S.record_key)
+                      k kk;
+      related_value_inj (V_dval gp.vegp_v)
+                        r.S.record_value
+                        (DVal d)
+                        vv
+
+////////////////////////////////////////////////////////////////////////////////
+// VPUT
+////////////////////////////////////////////////////////////////////////////////
+
+
+let update_entry #vcfg
+                 (i_record:IStore.vstore_entry vcfg)
+                 (v:Veritas.Record.value_type_of (IStore.VStoreE?.k i_record))
+  : IStore.vstore_entry vcfg
+  = let IStore.VStoreE kk _ am l_in_store r_in_store p = i_record in
+    IStore.VStoreE kk v am l_in_store r_in_store p
+
+let istore_upd_value #vcfg
+                     (st:IStore.vstore vcfg)
+                     (s:IStore.inuse_slot_id st)
+                     (d:Veritas.Record.value_type_of (IStore.stored_key st s))
+  : Lemma
+    (requires
+      Some? (IStore.get_slot st s))
+    (ensures (
+      let Some e = IStore.get_slot st s in
+      IStore.update_value st s d `Seq.equal`
+      Seq.upd st s (Some (update_entry e d))))
+    [SMTPat (IStore.update_value st s d)]
+  = let open IStore in
+    let st' = IStore.update_value st s d in
+    //just need to trigger a rewrite get_slot into seq.index
+    assert (forall i. i <> s ==> get_slot st i == get_slot st' i /\ Seq.index st i == Seq.index st' i)
+
+let related_vput (#vcfg: _)
+                 (tsm:S.thread_state_model)
+                 (vtls:I.vtls vcfg)
+                 (v:S_Types.vlog_entry { S_Types.Ve_Put? v })
+  : Lemma
+    (requires
+      Some? (lift_log_entry #vcfg v) /\
+      related_states tsm vtls /\
+      I.Valid? vtls)
+    (ensures (
+      let open S_Types in
+      let open IL in
+      let gp = Ve_Put?._0 v in
+      let Some (Put_S s k d) = lift_log_entry #vcfg v in
+      (S.vput_model tsm gp.vegp_s gp.vegp_k (V_dval gp.vegp_v))
+        `related_states`
+      (I.vput s k d vtls)))
+   = let open Veritas.Record in
+     let open S_Types in
+     let open IL in
+     let open S in
+     let gp = Ve_Put?._0 v in
+     let Some (Put_S s k d) = lift_log_entry #vcfg v in
+     related_lift_vlog_entry_get_put #vcfg gp;
+     let tsm' = S.vput_model tsm gp.vegp_s gp.vegp_k (V_dval gp.vegp_v) in
+     let vtls' = I.vput s k d vtls in
+     let I.Valid id st clock hadd hevict = vtls in
+     match model_get_record tsm gp.vegp_s with
+     | None -> ()
+     | Some r ->
+       let Some entry = IStore.get_slot st s in
+       let IStore.VStoreE kk vv am l_in_store r_in_store p = entry in
+       related_key_inj gp.vegp_k (r.S.record_key)
+                      k kk;
+       if k <> kk then ()
+       else istore_upd_value st s (DVal d)
+
+////////////////////////////////////////////////////////////////////////////////
+// VADDM
+////////////////////////////////////////////////////////////////////////////////
+
+let vaddm_basic_preconditions tsm s_s s_k s_v s_s' s_k' s_v'
+                              s_mv' s_d s_dh' s_h
+                              #vcfg (vtls:I.vtls vcfg{I.Valid? vtls})
+                              i_s i_k i_v i_s' i_k' i_v'
+                              i_mv' i_d i_dh' i_h
+  = let st = (I.thread_store vtls) in
+    related_states tsm vtls /\
+    related_slots #vcfg s_s i_s /\
+    related_key s_k i_k /\
+    related_value s_v i_v /\
+    related_slots #vcfg s_s' i_s' /\
+    related_key s_k' i_k' /\
+    related_value s_v' i_v' /\
+    (S.is_proper_descendent s_k s_k' /\
+     Some? (S.model_get_record tsm s_s') /\
+     S.is_value_of s_k s_v /\
+     (let r = Some?.v (S.model_get_record tsm s_s') in
+      r.S.record_key == s_k' /\
+      r.S.record_value == s_v') /\
+    Some s_mv' == S.to_merkle_value s_v' /\
+    s_d == S.desc_dir s_k s_k' /\
+    s_dh' == S.desc_hash_dir s_mv' s_d /\
+    s_h == S.hashfn s_v) /\
+    (i_s <> i_s' /\
+     not (IStore.empty_slot st i_s') /\
+     BinTree.is_proper_desc i_k i_k' /\
+     not (IStore.inuse_slot st i_s) /\
+     Record.is_value_of i_k i_v /\
+     IStore.stored_key st i_s' == i_k' /\
+     IStore.stored_value st i_s' == i_v' /\
+     i_mv'== Veritas.Record.to_merkle_value i_v' /\
+     i_d == Veritas.BinTree.desc_dir i_k i_k' /\
+     i_dh' == Veritas.Record.desc_hash_dir i_mv' i_d /\
+     i_h == Veritas.Hash.hashfn i_v)
+
+let related_vaddm_no_child tsm s_s s_k s_v s_s' s_k' s_v' s_mv' s_d s_dh' s_h
+                           #vcfg (vtls:I.vtls vcfg{I.Valid? vtls})
+                           i_s i_k i_v i_s' i_k' i_v' i_mv' i_d i_dh' i_h
+  : Lemma
+    (requires vaddm_basic_preconditions
+                   tsm s_s s_k s_v s_s' s_k' s_v'
+                   s_mv' s_d s_dh' s_h
+                   vtls i_s i_k i_v i_s' i_k' i_v'
+                   i_mv' i_d i_dh' i_h /\
+              S_Types.Dh_vnone? s_dh')
+    (ensures
+      (S.vaddm_model tsm s_s S_Types.({record_key = s_k; record_value = s_v}) s_s'
+        `related_states`
+      (I.vaddm i_s (i_k, i_v) i_s' vtls)))
+  = let open Veritas.Record in
+    let open S_Types in
+    let open IL in
+    let open S in
+    related_key_proper_descendent s_k s_k' i_k i_k';
+    let tsm' =
+      S.vaddm_model
+        tsm
+        s_s
+        S_Types.({record_key = s_k; record_value = s_v})
+        s_s'
+    in
+    let vtls' = I.vaddm i_s (i_k, i_v) i_s' vtls in
+    let st = (I.thread_store vtls) in
+    let s_r' = Some?.v (S.model_get_record tsm s_s') in
+    let Some i_r' = IStore.get_slot st i_s' in
+    related_hashfn s_v i_v;
+    related_desc_hash_dir s_mv' s_d i_mv' i_d;
+    assert (i_dh' == Empty);
+    related_init_value s_k i_k;
+    if s_v = S.init_value s_k
+    then (
+      assert (i_v = Veritas.Record.init_value i_k);
+      points_to_some_slot_related tsm st s_s' s_d i_d;
+      if S.points_to_some_slot tsm s_s' s_d
+      then ()
+      else (
+        madd_to_store_related tsm st s_s s_k s_v s_s' s_d i_s i_k i_v i_s' i_d;
+        let tsm1 = S.model_madd_to_store tsm s_s s_k s_v s_s' s_d in
+        let st1 = IStore.madd_to_store st i_s i_k i_v i_s' i_d in
+        assert (related_stores tsm1.S.model_store st1);
+
+        related_update_merkle_value
+                  (S_Types.V_mval?._0 s_v') s_d s_k s_h
+                  (Record.MVal?.v i_v') i_d i_k i_h false
+      )
+    )
+    else (
+      assert (i_v <> Veritas.Record.init_value i_k)
+    )
+
+let related_vaddm_some_child tsm s_s s_k s_v s_s' s_k' s_v' s_mv' s_d s_dh' s_h
+                           #vcfg (vtls:I.vtls vcfg{I.Valid? vtls})
+                           i_s i_k i_v i_s' i_k' i_v' i_mv' i_d i_dh' i_h
+  : Lemma
+    (requires vaddm_basic_preconditions
+                   tsm s_s s_k s_v s_s' s_k' s_v'
+                   s_mv' s_d s_dh' s_h
+                   vtls i_s i_k i_v i_s' i_k' i_v'
+                   i_mv' i_d i_dh' i_h /\
+              S_Types.Dh_vsome? s_dh')
+    (ensures
+      (S.vaddm_model tsm s_s S_Types.({record_key = s_k; record_value = s_v}) s_s'
+        `related_states`
+      (I.vaddm i_s (i_k, i_v) i_s' vtls)))
+  = let open Veritas.Record in
+    let open S_Types in
+    let open IL in
+    let open S in
+    related_key_proper_descendent s_k s_k' i_k i_k';
+    let tsm' =
+      S.vaddm_model
+        tsm
+        s_s
+        S_Types.({record_key = s_k; record_value = s_v})
+        s_s'
+    in
+    let vtls' = I.vaddm i_s (i_k, i_v) i_s' vtls in
+    let st = (I.thread_store vtls) in
+    let s_r' = Some?.v (S.model_get_record tsm s_s') in
+    let Some i_r' = IStore.get_slot st i_s' in
+    related_hashfn s_v i_v;
+    related_desc_hash_dir s_mv' s_d i_mv' i_d;
+    let Dh_vsome {dhd_key=s_k2; dhd_h=s_h2; evicted_to_blum = s_b2} = s_dh' in
+    let Desc i_k2 i_h2 i_b2 = i_dh' in
+    related_key_inj s_k s_k2 i_k i_k2;
+    if s_k2 = s_k
+    then (
+       points_to_some_slot_related tsm st s_s' s_d i_d;
+       if not (s_h2 = s_h && s_b2 = Vfalse)
+       then ()
+       else if points_to_some_slot tsm s_s' s_d
+       then ()
+       else (
+         madd_to_store_related tsm st s_s s_k s_v s_s' s_d i_s i_k i_v i_s' i_d
+       )
+    )
+    else (
+      related_init_value s_k i_k;
+      if s_v <> S.init_value s_k
+      then ()
+      else (
+        related_key_proper_descendent s_k2 s_k i_k2 i_k;
+        if not (S.is_proper_descendent s_k2 s_k)
+        then ()
+        else (
+          let Some s_mv = S.to_merkle_value s_v in
+          let s_d2 = S.desc_dir s_k2 s_k in
+          let Record.MVal i_mv = i_v in
+          let i_d2 = BinTree.desc_dir i_k2 i_k in
+          assert (related_desc_dir s_d2 i_d2);
+          related_update_merkle_value
+            s_mv s_d2 s_k2 s_h2
+            i_mv i_d2 i_k2 i_h2 i_b2;
+          let i_mv_upd = Verifier.update_merkle_value i_mv i_d2 i_k2 i_h2 i_b2 in
+          let s_mv_upd = S.update_merkle_value s_mv s_d2 s_k2 s_h2 (s_b2=Vtrue) in
+          related_update_merkle_value
+            s_mv' s_d s_k s_h
+            i_mv' i_d i_k i_h false;
+          let i_v'_upd = Verifier.update_merkle_value i_mv' i_d i_k i_h false in
+          let s_v'_upd = S.update_merkle_value s_mv' s_d s_k s_h false in
+          points_to_some_slot_related
+            tsm st s_s' s_d i_d;
+          if S.points_to_some_slot tsm s_s' s_d
+          then
+            madd_to_store_split_related tsm st
+              s_s s_k (V_mval s_mv_upd) s_s' s_d s_d2
+              i_s i_k (MVal i_mv_upd) i_s' i_d i_d2
+          else
+            madd_to_store_related tsm st
+               s_s s_k (V_mval s_mv_upd) s_s' s_d
+               i_s i_k (MVal i_mv_upd) i_s' i_d
+        )
+      )
+    )
+
+
+let related_vaddm (#vcfg: _)
+                  (tsm:S.thread_state_model)
+                  (vtls:I.vtls vcfg)
+                  (v:S_Types.vlog_entry)
+  : Lemma
+    (requires
+      S_Types.Ve_AddM? v == true /\
+      Some? (lift_log_entry #vcfg v) == true /\
+      related_states tsm vtls /\
+      I.Valid? vtls == true)
+    (ensures (
+      let open S_Types in
+      let open IL in
+      let addm = Ve_AddM?._0 v in
+      let Some (AddM_S s r s') = lift_log_entry #vcfg v in
+      (S.vaddm_model tsm addm.veam_s addm.veam_r addm.veam_s2
+        `related_states`
+      (I.vaddm s r s' vtls))))
+  = let open Veritas.Record in
+    let open S_Types in
+    let open IL in
+    let open S in
+    let addm = Ve_AddM?._0 v in
+    let Some (AddM_S i_s i_r i_s') = lift_log_entry #vcfg v in
+    related_lift_log_entry_addm #vcfg v;
+    let s_s = addm.veam_s in
+    let s_r = addm.veam_r in
+    let s_s' = addm.veam_s2  in
+    let tsm' = S.vaddm_model tsm s_s s_r s_s' in
+    let vtls' = I.vaddm i_s i_r i_s' vtls in
+    let I.Valid id st clock hadd hevict = vtls in
+    match model_get_record tsm s_s' with
+    | None -> ()
+    | Some s_r' ->
+      assert (not (IStore.empty_slot st i_s'));
+      let Some i_r' = IStore.get_slot st i_s' in
+      assert (related_record s_r' i_r');
+      let s_k = addm.veam_r.S_Types.record_key in
+      let s_v = addm.veam_r.S_Types.record_value in
+      let s_k' = s_r'.record_key in
+      let s_v' = s_r'.record_value in
+      let i_k, i_v = i_r in
+      let i_k' = IStore.stored_key st i_s' in
+      let i_v' = IStore.stored_value st i_s' in
+      if i_s = i_s'
+      then (
+        assert (vtls' == I.Failed);
+        assert (tsm'.model_failed)
+        //At the TSM level, we do not explicitly check that s <> s'
+        //but it follows anyway, since if s' is not in the store it fails
+        //and if s' is in the store then s must not be in the store
+      ) else (
+        related_key_proper_descendent s_k s_k' i_k i_k';
+        if not (S.is_proper_descendent s_k s_k')
+        then ()
+        else if Some? (model_get_record tsm s_s)
+        then ()
+        else (
+          value_of_related s_k s_v i_k i_v;
+          if not (S.is_value_of s_k s_v)
+          then ()
+          else (
+            assert (Veritas.Record.is_value_of i_k i_v);
+            assert (Veritas.Record.MVal? i_v');
+            assert (related_value s_v' i_v');
+            assert (S_Types.V_mval? s_v');
+            let i_mv' = Veritas.Record.to_merkle_value i_v' in
+            let i_d = Veritas.BinTree.desc_dir i_k i_k' in
+            let i_dh' = Veritas.Record.desc_hash_dir i_mv' i_d in
+            let i_h = Veritas.Hash.hashfn i_v in
+            let Some s_mv' = S.to_merkle_value s_v' in
+            let s_d = S.desc_dir s_k s_k' in
+            let s_dh' = S.desc_hash_dir s_mv' s_d in
+            let s_h = S.hashfn s_v in
+            related_hashfn s_v i_v;
+            assert (related_hashes (bitvec_of_u256 s_h) i_h);
+            related_desc_hash_dir s_mv' s_d i_mv' i_d;
+            match s_dh' with
+            | S_Types.Dh_vnone _ ->
+              related_vaddm_no_child
+                tsm s_s s_k s_v s_s' s_k' s_v' s_mv' s_d s_dh' s_h
+              vtls i_s i_k i_v i_s' i_k' i_v' i_mv' i_d i_dh' i_h
+            | _ ->
+              related_vaddm_some_child
+                tsm s_s s_k s_v s_s' s_k' s_v' s_mv' s_d s_dh' s_h
+              vtls i_s i_k i_v i_s' i_k' i_v' i_mv' i_d i_dh' i_h
+          )
+        )
+      )
+
+////////////////////////////////////////////////////////////////////////////////
+// vaddb
+////////////////////////////////////////////////////////////////////////////////
 
 let related_vaddb (#vcfg: _)
                   (tsm:S.thread_state_model)
@@ -1159,46 +1206,6 @@ let related_vevictm (#vcfg: _)
 // vevictb
 ////////////////////////////////////////////////////////////////////////////////
 
-let timestamp_lt_related  (s_t s_t':S_Types.timestamp)
-                          (i_t i_t':MSH.timestamp)
-  : Lemma
-    (requires
-      related_clocks s_t i_t /\
-      related_clocks s_t' i_t')
-    (ensures
-      MSH.ts_lt i_t i_t' <==>
-      S.timestamp_lt s_t s_t')
-    [SMTPat (related_clocks s_t i_t);
-     SMTPat (related_clocks s_t' i_t')]
-  = admit()
-
-let is_root_related (s_k:_) (i_k:Veritas.Key.key)
-  : Lemma
-    (requires
-      related_key s_k i_k)
-    (ensures
-      S.is_root s_k <==> i_k=BinTree.Root)
-    [SMTPat (related_key s_k i_k);
-     SMTPat (S.is_root s_k)]
-  = admit()
-
-let model_update_hash_related (s_h:_) (s_k:_) (s_v:_) (s_t:_) (s_j:_)
-                              (i_h:_) (i_k:_) (i_v:_) (i_t:_) (i_j:_)
-  : Lemma
-    (requires
-      related_hashes s_h i_h /\
-      related_key s_k i_k /\
-      related_value s_v i_v /\
-      related_thread_id s_j i_j /\
-      related_clocks s_t i_t)
-    (ensures (
-      let open S_Types in
-      related_hashes
-        (S.model_update_hash s_h ({record_key=s_k; record_value=s_v}) s_t s_j)
-        (MultiSetHash.ms_hashfn_upd (MSH.MHDom (i_k, i_v) i_t i_j) i_h)))
-    [SMTPat (S.model_update_hash s_h ({S_Types.record_key=s_k; S_Types.record_value=s_v}) s_t s_j);
-    SMTPat (MultiSetHash.ms_hashfn_upd (MSH.MHDom (i_k, i_v) i_t i_j) i_h)]
-  = admit()
 
 let related_sat_evictb_checks (#vcfg: _)
                               (tsm:S.thread_state_model)
@@ -1240,7 +1247,7 @@ let related_vevictb (#vcfg: _)
       let open IL in
       let { veeb_s = s_s; veeb_t = s_t} = Ve_EvictB?._0 v in
       let Some (EvictB_S i_s i_t) = lift_log_entry #vcfg v in
-      S.vevictb_model tsm s_s s_t z_thread_id
+      S.vevictb_model tsm s_s s_t
         `related_states`
       I.vevictb i_s i_t vtls))
   = ()
